src/Iris/Std/FiniteMapInst.lean
@@ -4,6 +4,7 @@ Released under Apache 2.0 license as described in the file LICENSE.
 Authors: Zongyuan Liu
 -/
 import Iris.Std.FiniteMap
+import Iris.Std.List
 import Std
 
 /-! ## FiniteMap Instance for Std.ExtTreeMap
@@ -18,22 +19,22 @@ which is a balanced binary search tree implementation.
 namespace Iris.Std
 
 /-- Instance of FiniteMap for Std.ExtTreeMap. -/
-instance {K : Type _} [Ord K] [Std.TransCmp (α := K) compare] [Std.LawfulEqCmp (α := K) compare] [DecidableEq K]:
-    FiniteMap (Std.ExtTreeMap K) K where
+instance {K : Type u} [Ord K] [Std.TransCmp (α := K) compare] [Std.LawfulEqCmp (α := K) compare] [DecidableEq K]:
+    FiniteMap K (Std.ExtTreeMap K) where
   get? m k := m.get? k
   insert m k v := m.insert k v
   delete m k := m.erase k
   empty := Std.ExtTreeMap.empty
   toList m := m.toList
-  ofList l := Std.ExtTreeMap.ofList l
-  fold := sorry
+  ofList l := Std.ExtTreeMap.ofList l.reverse
+  fold := fun f init m => m.foldr f init
 
 namespace FiniteMapInst
 
 variable {K : Type _} [Ord K] [Std.TransCmp (α := K) compare] [Std.LawfulEqCmp (α := K) compare] [DecidableEq K]
 
 /-- The FiniteMapLaws instance for ExtTreeMap. -/
-instance : FiniteMapLaws (Std.ExtTreeMap K) K where
+instance : FiniteMapLaws K (Std.ExtTreeMap K) where
   map_eq := by
     intro m₁ m₂ h
     apply Std.ExtTreeMap.ext_getElem?
@@ -63,64 +64,353 @@ instance : FiniteMapLaws (Std.ExtTreeMap K) K where
     trivial
 
   lookup_union := by
-    intro m₁ m₂ k
-    simp [FiniteMap.get?]
-    sorry
+    intro V m₁ m₂ k
+    simp only [FiniteMap.get?, Union.union, FiniteMap.union]
+    have h : ∀ (l : List (K × V)) (hnodup : (l.map Prod.fst).Nodup) (m : Std.ExtTreeMap K V compare),
+        (l.foldl (fun (acc: Std.ExtTreeMap K V compare) (x : K × V) => (Std.ExtTreeMap.insert acc x.fst x.snd: Std.ExtTreeMap K V compare)) m).get? k =
+        (l.lookup k).orElse (fun _ => m.get? k) := by
+      intro l hnodup m
+      induction l generalizing m with
+      | nil =>
+        simp [List.foldl, List.lookup, Option.orElse]
+      | cons p tail ih =>
+        obtain ⟨k', v'⟩ := p
+        simp only [List.foldl]
+        rw [List.map_cons, List.nodup_cons] at hnodup
+        rw [ih hnodup.2]
+        simp only [List.lookup]
+        by_cases h : k = k'
+        · subst h
+          simp
+          have hlookup_none : List.lookup k tail = none := by
+            cases hlookup : List.lookup k tail with
+            | none => rfl
+            | some v =>
+              exfalso
+              have hmem : (k, v) ∈ tail := Iris.Std.list_lookup_some_mem k v tail hlookup
+              have : k ∈ tail.map Prod.fst := by
+                simp
+                exact ⟨v, hmem⟩
+              exact hnodup.1 this
+          simp [hlookup_none]
+        · simp [Std.ExtTreeMap.getElem?_insert]
+          have heq : (k == k') = false := by
+            simp
+            intro heq_k_k'
+            exact h heq_k_k'
+          rw [heq]
+          have : k' ≠ k := fun heq_contr => h heq_contr.symm
+          simp [if_neg this]
+
+    have nodup : (m₁.toList.map Prod.fst).Nodup := by
+      rw [Std.ExtTreeMap.map_fst_toList_eq_keys]
+      exact Std.ExtTreeMap.nodup_keys
+    show (m₁.toList.foldl (fun acc x => acc.insert x.fst x.snd) m₂).get? k = _
+    rw [h m₁.toList nodup m₂]
+
+    congr 1
+    cases hlookup : m₁.toList.lookup k with
+    | none =>
+      cases hget : m₁.get? k with
+      | none => rfl
+      | some v =>
+        exfalso
+        have hmem : (k, v) ∈ m₁.toList :=
+          Std.ExtTreeMap.mem_toList_iff_getElem?_eq_some.mpr hget
+        have : m₁.toList.lookup k = some v :=
+          Iris.Std.list_mem_lookup_some k v _ nodup hmem
+        rw [hlookup] at this
+        contradiction
+    | some v =>
+      have hmem : (k, v) ∈ m₁.toList :=
+        Iris.Std.list_lookup_some_mem k v _ hlookup
+      have : m₁.get? k = some v :=
+        Std.ExtTreeMap.mem_toList_iff_getElem?_eq_some.mp hmem
+      rw [this]
 
   lookup_difference := by
-    intro m₁ m₂ k
-    simp [FiniteMap.get?]
-    sorry
+    intro V m₁ m₂ k
+    simp only [FiniteMap.get?, SDiff.sdiff, FiniteMap.difference, FiniteMap.ofList, FiniteMap.toList]
+    rw [Std.ExtTreeMap.ofList_eq_insertMany_empty]
+    by_cases hm₂ : m₂.get? k = none
+    · simp only [hm₂, Option.isSome_none]
+      simp
+      cases hm₁ : m₁.get? k with
+      | none =>
+        have hk_not_in : k ∉ ((List.filter (fun x => m₂[x.fst]?.isNone) m₁.toList).reverse.map Prod.fst) := by
+          intro hmem
+          rw [List.mem_map] at hmem
+          obtain ⟨⟨k', v'⟩, hmem_rev, hkeq⟩ := hmem
+          simp at hkeq
+          subst hkeq
+          have hmem_filter : (k', v') ∈ List.filter (fun x => m₂[x.fst]?.isNone) m₁.toList :=
+            List.mem_reverse.mp hmem_rev
+          rw [List.mem_filter] at hmem_filter
+          obtain ⟨hmem_toList, _⟩ := hmem_filter
+          have hcontr : m₁.get? k' = some v' := Std.ExtTreeMap.mem_toList_iff_getElem?_eq_some.mp hmem_toList
+          rw [hm₁] at hcontr
+          contradiction
+        have hk_contains : ((List.filter (fun x => m₂[x.fst]?.isNone) m₁.toList).reverse.map Prod.fst).contains k = false := by
+          cases h : ((List.filter (fun x => m₂[x.fst]?.isNone) m₁.toList).reverse.map Prod.fst).contains k
+          · rfl
+          · rw [List.contains_iff_mem] at h
+            exact absurd h hk_not_in
+        show ((∅ : Std.ExtTreeMap K V compare).insertMany (List.filter (fun x => m₂[x.fst]?.isNone) m₁.toList).reverse)[k]? = m₁[k]?
+        rw [Std.ExtTreeMap.getElem?_insertMany_list_of_contains_eq_false hk_contains]
+        show (∅ : Std.ExtTreeMap K V compare)[k]? = m₁[k]?
+        simp only [Std.ExtTreeMap.getElem?_empty]
+        exact hm₁.symm
+      | some v₁ =>
+        have hmem_toList : (k, v₁) ∈ m₁.toList :=
+          Std.ExtTreeMap.mem_toList_iff_getElem?_eq_some.mpr hm₁
+        have hfilter : (m₂.get? k).isNone = true := by
+          rw [hm₂]
+          rfl
+        have hmem_filter : (k, v₁) ∈ List.filter (fun x => m₂[x.fst]?.isNone) m₁.toList := by
+          rw [List.mem_filter]
+          simp only
+          exact ⟨hmem_toList, hfilter⟩
+        have hmem_rev : (k, v₁) ∈ (List.filter (fun x => m₂[x.fst]?.isNone) m₁.toList).reverse :=
+          List.mem_reverse.mpr hmem_filter
+        have hdistinct : (List.filter (fun x => m₂[x.fst]?.isNone) m₁.toList).reverse.Pairwise (fun a b => ¬compare a.1 b.1 = .eq) := by
+          rw [List.pairwise_reverse]
+          have hdist_toList : m₁.toList.Pairwise (fun a b => ¬compare a.1 b.1 = .eq) :=
+            Std.ExtTreeMap.distinct_keys_toList
+          have hdist_filter : (List.filter (fun x => m₂[x.fst]?.isNone) m₁.toList).Pairwise (fun a b => ¬compare a.1 b.1 = .eq) := by
+            apply List.Pairwise.filter
+            exact hdist_toList
+          apply hdist_filter.imp
+          intro a b h heq
+          have : compare a.1 b.1 = .eq := by
+            have hsym : compare b.1 a.1 = .eq → compare a.1 b.1 = .eq := by
+              intro hba
+              rw [Std.LawfulEqCmp.compare_eq_iff_eq] at hba ⊢
+              exact hba.symm
+            exact hsym heq
+          exact h this
+        have hcmp_eq : compare k k = .eq := Std.LawfulEqCmp.compare_eq_iff_eq.mpr rfl
+        show ((∅ : Std.ExtTreeMap K V compare).insertMany (List.filter (fun x => m₂[x.fst]?.isNone) m₁.toList).reverse)[k]? = m₁[k]?
+        rw [Std.ExtTreeMap.getElem?_insertMany_list_of_mem hcmp_eq hdistinct hmem_rev]
+        exact hm₁.symm
+    · cases hget : m₂.get? k with
+      | none => contradiction
+      | some v₂ =>
+        simp only [Option.isSome_some, ite_true]
+        have hk_not_in : k ∉ ((List.filter (fun x => (m₂.get? x.fst).isNone) m₁.toList).reverse.map Prod.fst) := by
+          intro hmem
+          rw [List.mem_map] at hmem
+          obtain ⟨⟨k', v'⟩, hmem_rev, hkeq⟩ := hmem
+          simp at hkeq
+          subst hkeq
+          have hmem_filter : (k', v') ∈ List.filter (fun x => (m₂.get? x.fst).isNone) m₁.toList :=
+            List.mem_reverse.mp hmem_rev
+          rw [List.mem_filter] at hmem_filter
+          obtain ⟨_, hfilter⟩ := hmem_filter
+          simp only [Option.isNone_iff_eq_none] at hfilter
+          rw [hget] at hfilter
+          contradiction
+        have hk_contains : ((List.filter (fun x => (m₂.get? x.fst).isNone) m₁.toList).reverse.map Prod.fst).contains k = false := by
+          cases h : ((List.filter (fun x => (m₂.get? x.fst).isNone) m₁.toList).reverse.map Prod.fst).contains k
+          · rfl
+          · rw [List.contains_iff_mem] at h
+            exact absurd h hk_not_in
+        show ((∅ : Std.ExtTreeMap K V compare).insertMany (List.filter (fun x => (m₂.get? x.fst).isNone) m₁.toList).reverse)[k]? = none
+        rw [Std.ExtTreeMap.getElem?_insertMany_list_of_contains_eq_false hk_contains]
+        rfl
 
   ofList_nil := by
     simp [FiniteMap.ofList]
 
   ofList_cons := by
-    intro k v l
+    intro k v l l_1
     simp only [FiniteMap.ofList, FiniteMap.insert]
-    sorry
+    rw [List.reverse_cons, Std.ExtTreeMap.ofList_eq_insertMany_empty, Std.ExtTreeMap.ofList_eq_insertMany_empty, Std.ExtTreeMap.insertMany_append, Std.ExtTreeMap.insertMany_list_singleton]
 
-  fold_empty := by sorry
+  map_to_list_spec := by
+    intro V m
+    constructor
+    · simp only [FiniteMap.toList]
+      have hdistinct : m.toList.Pairwise (fun a b => ¬compare a.1 b.1 = .eq) :=
+        Std.ExtTreeMap.distinct_keys_toList
+      apply hdistinct.imp
+      intro a b hne heq
+      subst heq
+      have : compare a.1 a.1 = .eq := Std.LawfulEqCmp.compare_eq_iff_eq.mpr rfl
+      exact hne this
+    · intro i x
+      simp only [FiniteMap.toList, FiniteMap.get?]
+      exact Std.ExtTreeMap.mem_toList_iff_getElem?_eq_some
 
-  fold_fmap_ind := by sorry
+  map_ind := by
+    intros V P H0 Hind m
+
+    have hm : m = Std.ExtTreeMap.insertMany ∅ (Std.ExtTreeMap.toList m).reverse := by
+      apply Std.ExtTreeMap.ext_getElem?
+      intro k
+      cases hget : m[k]? with
+      | none =>
+        have hk_not_in : k ∉ (m.toList.reverse.map Prod.fst) := by
+          intro hmem
+          rw [List.mem_map] at hmem
+          obtain ⟨⟨k', v'⟩, hmem_rev, hkeq⟩ := hmem
+          simp at hkeq
+          subst hkeq
+          have hmem_toList : (k', v') ∈ m.toList := List.mem_reverse.mp hmem_rev
+          have : m[k']? = some v' := Std.ExtTreeMap.mem_toList_iff_getElem?_eq_some.mp hmem_toList
+          rw [hget] at this
+          contradiction
+        have hk_contains : (m.toList.reverse.map Prod.fst).contains k = false := by
+          cases h : (m.toList.reverse.map Prod.fst).contains k
+          · rfl
+          · rw [List.contains_iff_mem] at h
+            exact absurd h hk_not_in
+        rw [Std.ExtTreeMap.getElem?_insertMany_list_of_contains_eq_false hk_contains]
+        rfl
+      | some v =>
+        have hmem_toList : (k, v) ∈ m.toList :=
+          Std.ExtTreeMap.mem_toList_iff_getElem?_eq_some.mpr hget
+        have hmem_rev : (k, v) ∈ m.toList.reverse := List.mem_reverse.mpr hmem_toList
+        have hdistinct : m.toList.Pairwise (fun a b => ¬compare a.1 b.1 = .eq) :=
+          Std.ExtTreeMap.distinct_keys_toList
+        have hdistinct_rev : m.toList.reverse.Pairwise (fun a b => ¬compare a.1 b.1 = .eq) := by
+          rw [List.pairwise_reverse]
+          apply hdistinct.imp
+          intro a b h
+          intro heq
+          have : compare a.1 b.1 = .eq := by
+            have hsym : compare b.1 a.1 = .eq → compare a.1 b.1 = .eq := by
+              intro h
+              rw [Std.LawfulEqCmp.compare_eq_iff_eq] at h ⊢
+              exact h.symm
+            exact hsym heq
+          exact h this
+        have hcmp_eq : compare k k = .eq := Std.LawfulEqCmp.compare_eq_iff_eq.mpr rfl
+        have : ((∅ : Std.ExtTreeMap K V compare).insertMany m.toList.reverse)[k]? = some v :=
+          Std.ExtTreeMap.getElem?_insertMany_list_of_mem hcmp_eq hdistinct_rev hmem_rev
+        exact this.symm
+
+    rw [hm]
+
+    generalize hgen : (Std.ExtTreeMap.toList m) = l
+    have hdistinct : l.Pairwise (fun a b => ¬ compare a.1 b.1 = .eq) := by
+      rw [← hgen]
+      exact Std.ExtTreeMap.distinct_keys_toList
+    clear hgen hm m
+    induction l with
+    | nil =>
+      simp [Std.ExtTreeMap.insertMany_nil]
+      exact H0
+    | cons kv tail ih =>
+      obtain ⟨k, v⟩ := kv
+      simp
+      rw [Std.ExtTreeMap.insertMany_append]
+      simp
+
+      rw [List.pairwise_cons] at hdistinct
+      obtain ⟨hk_not_in_tail, htail_distinct⟩ := hdistinct
+
+      have hk_not_contains : (tail.reverse.map Prod.fst).contains k = false := by
+        apply Decidable.byContradiction
+        intro h
+        have h_true : (tail.reverse.map Prod.fst).contains k = true := by
+          cases h_dec : (tail.reverse.map Prod.fst).contains k
+          · exact absurd h_dec h
+          · rfl
+        rw [List.contains_iff_mem] at h_true
+        rw [List.mem_map] at h_true
+        obtain ⟨⟨k', v'⟩, hmem_rev, hkeq⟩ := h_true
+        simp at hkeq
+        have hmem_tail : (k', v') ∈ tail := List.mem_reverse.mp hmem_rev
+        have hk_neq : ¬ compare k k' = .eq := hk_not_in_tail (k', v') hmem_tail
+        have : compare k k' = .eq := by
+          rw [hkeq]
+          rw [Std.LawfulEqCmp.compare_eq_iff_eq]
+        exact hk_neq this
+
+      apply Hind
+      · show ((∅ : Std.ExtTreeMap K V compare).insertMany tail.reverse)[k]? = none
+        rw [Std.ExtTreeMap.getElem?_insertMany_list_of_contains_eq_false hk_not_contains]
+        rfl
+      · exact ih htail_distinct
 
 /-- The FiniteMapLawsSelf instance for ExtTreeMap. -/
-instance : FiniteMapLawsSelf (Std.ExtTreeMap K) K where
+instance : FiniteMapLawsSelf K (Std.ExtTreeMap K) where
   toList_filterMap := by
-    intro m f
-    simp [FiniteMap.toList, FiniteMap.filterMap, FiniteMap.ofList]
-    sorry
+    intro V m f
+    haveI : DecidableEq V := Classical.typeDecidableEq V
+    simp only [FiniteMap.toList, FiniteMap.filterMap, FiniteMap.ofList]
+
+    obtain H := FiniteMapLaws.map_to_list_to_map (M := (Std.ExtTreeMap K)) (K := K) (V := V) (l := (List.filterMap (fun kv => Option.map (fun x => (kv.fst, x)) (f kv.snd)) m.toList))
+
+    simp only [FiniteMap.toList, FiniteMap.ofList] at H
+    apply H
+    rw [List.map_filterMap]
+    have eq_goal : (List.filterMap (fun x => Option.map Prod.fst (Option.map (fun x_1 => (x.fst, x_1)) (f x.snd))) m.toList) =
+                   (List.filterMap (fun x => Option.map (fun _ => x.fst) (f x.snd)) m.toList) := by
+      congr 1
+      ext x
+      rw [Option.map_map]
+      rfl
+    rw [eq_goal]
+    have nodup_keys : (m.toList.map Prod.fst).Nodup := by
+      rw [Std.ExtTreeMap.map_fst_toList_eq_keys]
+      exact Std.ExtTreeMap.nodup_keys
+    exact nodup_filterMap_of_nodup_keys m.toList f nodup_keys
 
   toList_filter := by
-    intro m φ
+    intro V m φ
     simp [FiniteMap.toList, FiniteMap.filter, FiniteMap.ofList]
-    sorry
+    haveI : DecidableEq V := Classical.typeDecidableEq V
+    obtain H := FiniteMapLaws.map_to_list_to_map (M := (Std.ExtTreeMap K)) (K := K) (V := V) (l := (List.filter (fun x => φ x.fst x.snd) m.toList))
 
-  toList_union_disjoint := by
-    intro m₁ m₂ h
-    simp [FiniteMap.toList]
-    sorry
+    simp only [FiniteMap.toList, FiniteMap.ofList] at H
+    apply H
 
-  toList_difference := by
-    intro m₁ m₂
-    simp [FiniteMap.toList]
-    sorry
+    have nodup_keys : (m.toList.map Prod.fst).Nodup := by
+      rw [Std.ExtTreeMap.map_fst_toList_eq_keys]
+      exact Std.ExtTreeMap.nodup_keys
+
+    exact nodup_map_fst_filter m.toList (fun x => φ x.fst x.snd) nodup_keys
 
 /-- The FiniteMapKmapLaws instance for ExtTreeMap with key type transformation. -/
 instance {K' : Type _} [Ord K'] [Std.TransCmp (α := K') compare] [Std.LawfulEqCmp (α := K') compare] [DecidableEq K'] :
-    FiniteMapKmapLaws (Std.ExtTreeMap K) (Std.ExtTreeMap K') K K' where
+    FiniteMapKmapLaws K K' (Std.ExtTreeMap K) (Std.ExtTreeMap K') where
   toList_kmap := by
-    intro f m hinj
+    intro V f m hinj
     simp [FiniteMap.toList, FiniteMap.kmap, FiniteMap.ofList]
-    sorry
+    haveI : DecidableEq V := Classical.typeDecidableEq V
+    obtain H := FiniteMapLaws.map_to_list_to_map (M := (Std.ExtTreeMap K')) (K := K') (V := V) (l := (List.map (fun x => (f x.fst, x.snd)) m.toList))
+
+    simp only [FiniteMap.toList, FiniteMap.ofList] at H
+    apply H
+
+    have nodup_keys : (m.toList.map Prod.fst).Nodup := by
+      rw [Std.ExtTreeMap.map_fst_toList_eq_keys]
+      exact Std.ExtTreeMap.nodup_keys
+
+    exact nodup_map_fst_map_injective m.toList f hinj nodup_keys
 
 /-- The FiniteMapSeqLaws instance for ExtTreeMap with Nat keys. -/
-instance {V' : Type _} [Std.TransCmp (α := Nat) compare] [Std.LawfulEqCmp (α := Nat) compare] :
+instance [Std.TransCmp (α := Nat) compare] [Std.LawfulEqCmp (α := Nat) compare] :
     FiniteMapSeqLaws (Std.ExtTreeMap Nat) where
   toList_map_seq := by
-    intro start l
+    intro V start l
     simp [FiniteMap.toList, FiniteMap.map_seq, FiniteMap.ofList]
-    sorry
+    haveI : DecidableEq V := Classical.typeDecidableEq V
+
+    have heq : List.mapIdx (fun i v => (start + i, v)) l = (List.range' start l.length).zip l :=
+      mapIdx_add_eq_zip_range' start l
+
+    rw [heq]
+
+    obtain H := FiniteMapLaws.map_to_list_to_map (M := (Std.ExtTreeMap Nat)) (K := Nat) (V := V) (l := ((List.range' start l.length).zip l))
+
+    simp only [FiniteMap.toList, FiniteMap.ofList] at H
+    apply H
+
+    -- The keys from range' are all distinct
+    rw [← heq]
+    exact nodup_map_fst_mapIdx_add start l
 
 end FiniteMapInst
 
